version with footprints in progress

examples/security/statefulEnc-multi-frame.fst
@@ -1,6 +1,6 @@
 (*--build-config
-    options:--admit_fsi Set --admit_fsi Seq;
-    other-files:../../lib/ext.fst ../../lib/set.fsi ../../lib/heap.fst ../../lib/st.fst ../../lib/seq.fsi
+    options:--admit_fsi Set --admit_fsi Seq --z3timeout 10;
+    other-files:../../lib/ext.fst ../../lib/set.fsi ../../lib/heap.fst ../../lib/st.fst ../../lib/seq.fsi ../../lib/list.fst
   --*)
 (* A standalone experiment corresponding to building a stateful encryption on
    top of a stateless one ... along the lines of StatefulLHAE on top of AEAD_GCM *)
@@ -8,7 +8,7 @@
 (* Still to do:
      Show that multiple instances do not overlap using footprints and dynamic frames
 *)
-module StatefulEncryption.MultiInstance
+module StatefulEncryption.MultiInstance.Frame
 open ST
 open Set
 open Heap
@@ -28,9 +28,15 @@ type Fresh (#a:Type) h0 (r:ref a) h1 = Heap.contains h1 r /\ not (Heap.contains 
 
 type Let (#a:Type) (x:a) (body: (y:a{y=x} -> Type)) = body x
 
+(* ------------------------------------------------------------ *)
+
 type plain
+assume val mk_plain: unit -> Tot plain
 type cipher
+assume val mk_cipher: unit -> Tot cipher
 type key
+assume val mk_key: unit -> Tot key
+
 
 type basicEntry =
   | Entry : p:plain -> c:cipher -> basicEntry
@@ -43,49 +49,105 @@ type decryptor =
 
 type paired (e:encryptor) (d:decryptor) = b2t (Enc.log e = Dec.log d)
 
-type both = ed:(encryptor * decryptor){paired (fst ed) (snd ed)}
+type bi =
+  | BI : e:encryptor -> d:decryptor{paired e d} -> bi
 
-val gen: unit -> St both
-  (requires (fun h -> True))
+let bi_refs (BI e d) = !{Enc.log e}
+
+type distinct_bi (b1:bi) (b2:bi) =
+  Set.Equal (Set.intersect (bi_refs b1) (bi_refs b2)) !{}
+
+type pairwise_distinct (s:list bi) =
+  forall b1 b2. List.mem b1 s /\ List.mem b2 s ==> (b1 = b2 \/ distinct_bi b1 b2)
+
+let basic_fp : ref (s:list bi{pairwise_distinct s}) = ref []
+
+type basic_fp_inv (h:heap) =
+  Heap.contains h basic_fp
+  /\ (forall bi.//{:pattern (List.mem bi (Heap.sel h basic_fp))}
+        List.mem bi (Heap.sel h basic_fp)
+         ==> (forall (a:Type) (r:ref a). //{:pattern (Heap.contains h r)}
+                Set.mem (Ref r) (bi_refs bi)
+                ==> Heap.contains h r /\ r =!= basic_fp))
+
+val gen: unit -> St bi
+  (requires (basic_fp_inv))
   (ensures (fun h0 b h1 ->
-      modifies !{} h0 h1
-      /\ Let (Enc.log (fst b)) (fun log ->
+      modifies !{basic_fp} h0 h1
+      /\ basic_fp_inv h1
+      /\ Heap.sel h1 basic_fp = b::Heap.sel h0 basic_fp
+      /\ Let (Enc.log (BI.e b)) (fun log ->
          Fresh h0 log h1
          /\ Heap.sel h1 log = emp)))
 let gen () =
-  let key : key = magic () in
+  let key = mk_key () in
   let log = ref emp in
-  (Enc log key, Dec log key)
+  let bi = BI (Enc log key) (Dec log key) in
+  basic_fp := bi::!basic_fp; //ghost
+  bi
+
+type enc_in_basic_fp (e:encryptor) (h:heap) =
+  exists d. paired e d /\ List.mem (BI e d) (Heap.sel h basic_fp)
+
+type dec_in_basic_fp (d:decryptor) (h:heap) =
+  exists e. paired e d /\ List.mem (BI e d) (Heap.sel h basic_fp)
+
+let in_basic_fp bi h = List.mem bi (Heap.sel h basic_fp)
 
 val enc : e:encryptor -> p:plain -> St cipher
-    (requires (fun h -> True))
+    (requires (fun h -> basic_fp_inv h /\ enc_in_basic_fp e h))
     (ensures (fun h0 c h1 ->
                 modifies !{Enc.log e} h0 h1
+                /\ basic_fp_inv h1
                 /\ Heap.contains h1 (Enc.log e)
                 /\ Heap.sel h1 (Enc.log e) = snoc (Heap.sel h0 (Enc.log e)) (Entry p c)))
-
 let enc e p =
-    let c : cipher = magic () in
+    let c = mk_cipher () in
     Enc.log e := snoc !(Enc.log e) (Entry p c);
     c
 
 assume val find_seq : #a:Type -> f:(a -> Tot bool) -> s:seq a
             -> Tot (o:option (i:nat{i < Seq.length s /\ f (Seq.index s i)}) { is_None o ==> (forall (i:nat{i < Seq.length s}). not (f (Seq.index s i)))})
 
+opaque logic type trigger (#a:Type) (x:a) = True
+
 val dec: d:decryptor -> c:cipher -> St (option plain)
-  (requires (fun h -> True))
+  (requires (fun h -> basic_fp_inv h /\ dec_in_basic_fp d h))
   (ensures (fun h0 p h1 ->
               modifies !{} h0 h1
+              /\ basic_fp_inv h1
               /\ (Let (Heap.sel h0 (Dec.log d))
                       (fun log ->
-                          (is_None p ==> (forall (i:nat{i < Seq.length log}). Entry.c (Seq.index log i) <> c))
-                          /\ (is_Some p ==> (exists (i:nat{i < Seq.length log}). Seq.index log i = Entry (Some.v p) c))))))
+                          (is_None p <==> (forall (i:nat{i < Seq.length log}).{:pattern (trigger i)} trigger i /\ Entry.c (Seq.index log i) <> c))
+                          /\ (is_Some p ==> (exists (i:nat{i < Seq.length log}).{:pattern (trigger i)} trigger i /\ Seq.index log i = Entry (Some.v p) c))))))
 let dec d c =
   let s = !(Dec.log d) in
   match find_seq (function Entry p c' -> c=c') s with
     | None -> None
-    | Some i -> Some (Entry.p (Seq.index s i))
+    | Some i ->
+      cut (trigger i);
+      Some (Entry.p (Seq.index s i))
 
+val test_basic_frame : b1:bi -> b2:bi{distinct_bi b1 b2} -> St unit
+    (requires (fun h -> basic_fp_inv h
+                    /\ in_basic_fp b1 h
+                    /\ in_basic_fp b2 h
+                    /\ Heap.sel h (Enc.log (BI.e b1)) = emp
+                    /\ Heap.sel h (Enc.log (BI.e b2)) = emp))
+    (ensures (fun h0 _ h1 ->
+                basic_fp_inv h1
+                /\ modifies (Set.union (bi_refs b1) (bi_refs b2)) h0 h1))
+
+let test_basic_frame b1 b2 =
+  let p1 = mk_plain () in
+  let p2 = mk_plain () in
+  let c1 = enc (BI.e b1) p1 in
+  let c2 = enc (BI.e b2) p2 in
+  let p1' = dec (BI.d b1) c1 in
+  let p2' = dec (BI.d b2) c2 in
+  cut (trigger 0);
+  assert (is_Some p1' /\ Some.v p1' = p1);
+  assert (is_Some p2' /\ Some.v p2' = p2)
 
 (* -------------------------------------------------------- *)
 type statefulEntry =
@@ -97,7 +159,6 @@ type st_encryptor =
 type st_decryptor =
   | StDec : log: ref (seq statefulEntry) -> ctr: ref nat -> key:decryptor -> st_decryptor
 
-
 type st_paired (enc:st_encryptor) (dec:st_decryptor) =
       StEnc.log enc = StDec.log dec
       /\ paired (StEnc.key enc) (StDec.key dec)
@@ -105,10 +166,26 @@ type st_paired (enc:st_encryptor) (dec:st_decryptor) =
       /\ StEnc.ctr enc <> StDec.ctr dec
       /\ StEnc.log enc =!= StEnc.ctr enc                      //These last four are needed because seq is abstract
       /\ StEnc.log enc =!= StDec.ctr dec                      //...
-      /\ (Enc.log (StEnc.key enc)) =!= StEnc.ctr enc            //...
-      /\ (Enc.log (StEnc.key enc)) =!= StDec.ctr dec           //and so potentially equal to nat ... TODO: make seq a new type
+      /\ (Enc.log (StEnc.key enc)) =!= StEnc.ctr enc          //...
+      /\ (Enc.log (StEnc.key enc)) =!= StDec.ctr dec          //and so potentially equal to nat ... TODO: make seq a new type
 
-type st_both = b:(st_encryptor * st_decryptor){st_paired (fst b) (snd b)}
+type sti =
+  | STI : e:st_encryptor -> d:st_decryptor{st_paired e d} -> sti
+
+
+let sti_refs (STI e d) =
+  Set.union !{StEnc.log e, StEnc.ctr e, StDec.ctr d}
+            (bi_refs (BI (StEnc.key e) (StDec.key d)))
+
+
+type distinct_sti (s1:sti) (s2:sti) =
+  Set.Equal (Set.intersect (sti_refs s1) (sti_refs s2)) Set.empty
+
+
+type pairwise_distinct_sti (s:list sti) =
+  forall s1 s2. List.mem s1 s /\ List.mem s2 s ==> (s1 = s2 \/ distinct_sti s1 s2)
+
+let st_fp : ref (s:list sti{pairwise_distinct_sti s}) = ref []
 
 assume val with_seqn : nat -> plain -> Tot plain
 
@@ -131,34 +208,59 @@ type st_inv (e:st_encryptor) (d:st_decryptor) (h:heap) =
             /\ Seq.index basic i = Entry (with_seqn i (StEntry.p st_en)) (StEntry.c st_en)))))))
 
 type st_enc_inv (e:st_encryptor) (h:heap) =
-  exists (d:st_decryptor). st_inv e d h
+  exists (d:st_decryptor). st_paired e d /\ st_inv e d h
 
 type st_dec_inv (d:st_decryptor) (h:heap) =
-  exists (e:st_encryptor). st_inv e d h
+  exists (e:st_encryptor). st_paired e d /\ st_inv e d h
+
+type st_fp_inv (h:heap) =
+   basic_fp_inv h
+   /\ Heap.contains h st_fp
+   /\ basic_fp =!= st_fp
+   /\ (forall sti.
+          List.mem sti (Heap.sel h st_fp)
+          ==> in_basic_fp (BI (StEnc.key (STI.e sti)) (StDec.key (STI.d sti))) h
+              /\ st_inv (STI.e sti) (STI.d sti) h
+              /\ (forall (a:Type) (r:ref a).
+                    Set.mem (Ref r) (sti_refs sti)
+                    ==> Heap.contains h r
+                        /\ r =!= basic_fp
+                        /\ r =!= st_fp))
 
 let refs_in_e (e:st_encryptor) = !{StEnc.log e, StEnc.ctr e, Enc.log (StEnc.key e)}
-
 let refs_in_d (d:st_decryptor) = !{StDec.log d, StDec.ctr d, Dec.log (StDec.key d)}
 
-val stateful_gen : unit -> St st_both
-  (requires (fun h -> True))
+val stateful_gen : unit -> St sti
+  (requires (st_fp_inv))
   (ensures (fun h0 b h1 ->
-              st_inv (fst b) (snd b) h1
-              /\ modifies !{} h0 h1
-              /\ (forall (a:Type) (r:ref a). Set.mem (Ref r) (Set.union (refs_in_e (fst b)) (refs_in_d (snd b)))
+              st_fp_inv h1
+              /\ Heap.sel h1 st_fp = b::Heap.sel h0 st_fp
+              /\ modifies !{basic_fp, st_fp} h0 h1
+              /\ (forall (a:Type) (r:ref a). Set.mem (Ref r) (sti_refs b)
                     ==> Fresh h0 r h1)))
 let stateful_gen () =
-  let e,d = gen () in
+  let BI e d = gen () in
   let l = ref emp in
   let w = ref 0 in
   let r = ref 0 in
-  (StEnc l w e, StDec l r d)
+  let sti = STI (StEnc l w e) (StDec l r d) in
+  st_fp := sti :: !st_fp; //ghost
+  sti
+
+let in_st_fp sti h = List.mem sti (Heap.sel h st_fp)
+
+type enc_in_st_fp (e:st_encryptor) (h:heap) =
+  exists d. st_paired e d /\ in_st_fp (STI e d) h
+
+type dec_in_st_fp (d:st_decryptor) (h:heap) =
+  exists e. st_paired e d /\ List.mem (STI e d) (Heap.sel h st_fp)
 
 val stateful_enc : e:st_encryptor -> p:plain -> St cipher
-  (requires (fun h -> st_enc_inv e h))
+  (requires (fun h -> st_fp_inv h /\ enc_in_st_fp e h))
   (ensures (fun h0 c h1 ->
-                    st_enc_inv e h1
-                 /\ modifies (refs_in_e e) h0 h1
+                  st_fp_inv h1
+                 /\
+                 modifies (refs_in_e e) h0 h1
                  /\ Heap.sel h1 (StEnc.log e) = snoc (Heap.sel h0 (StEnc.log e)) (StEntry (Heap.sel h0 (StEnc.ctr e)) p c)))
 
 let stateful_enc e p =
@@ -167,13 +269,16 @@ let stateful_enc e p =
   let c = enc (StEnc.key e) ip in
   StEnc.log e := snoc !(StEnc.log e) (StEntry i p c);
   StEnc.ctr e := i + 1;
+  let h1 = get () in
+  admitP(st_fp_inv h1);
   c
 
-val stateful_dec: ad:nat -> d:st_decryptor -> c:cipher -> St (option plain)
-  (requires (fun h -> st_dec_inv d h))
+(*val stateful_dec: ad:nat -> d:st_decryptor -> c:cipher -> St (option plain)
+  (requires (fun h -> st_fp_inv h /\ dec_in_st_fp d h))
   (ensures (fun h0 p h1 ->
-                st_dec_inv d h0
-                /\ st_dec_inv d h1
+                st_fp_inv h0
+                /\ dec_in_st_fp d h0 //repeating pre
+                /\ st_fp_inv h1
                 /\ modifies !{StDec.ctr d} h0 h1
                 /\ Let (Heap.sel h0 (StDec.ctr d)) (fun (r:nat{r=Heap.sel h0 (StDec.ctr d)}) ->
                    Let (Heap.sel h0 (StDec.log d)) (fun (log:seq statefulEntry{log=Heap.sel h0 (StDec.log d)}) ->
@@ -194,4 +299,4 @@ let stateful_dec ad d c =
            if i = ad
            then (StDec.ctr d := i + 1; Some q)
            else None
-      else None
+      else None*)
